# 1.6

### 78

##### 5

$p: $Randy works hard

$q: $Randy is a dull boy

$r: $Randy will not get the job

We have:

$1.p \qquad 2.p\rightarrow q\qquad 3.q\rightarrow r$

Then:

$p$	(premise1)

$\Rightarrow p\rightarrow q$	(premise2)

$\Rightarrow q$	(Modus Ponens using 1 and 2)

$\Rightarrow q\to r$	(premise3)

$\Rightarrow r$	(Modus Ponens)





##### 11

$Proof:$

$Case \;I:$

If the truth value of $q$ is True, then we can regard $q$ as a premise, then the problem can convert into that premises  $p_1,p_2,\dots,p_n,q$  and conclusion is $r$.

So, if the second statement is valid, the first is valid.

$Case \;II:$

Otherwise, $q$ is False. The first statement is already valid.



$Another Proof:$

|     $(p1\land p2\land ...\land p_n\land q)\rightarrow r$     |   $premise$   |
| :----------------------------------------------------------: | :-----------: |
|      $\lnot(p1\land p2\land ...\land p_n\land q)\lor r$      | $Implication$ |
|    $\lnot(p1\land p2\land ...\land p_n)\lor\lnot q\lor r$    | $DoMorgan's$  |
|  $\lnot(p1\land p2\land ...\land p_n)\lor( q\rightarrow r)$  | $Implication$ |
| $(p1\land p2\land ...\land p_n)\rightarrow( q\rightarrow r)$ | $Implication$ |



##### 15

a) correct	Universal Instantiation.

b) incorrect 	It's affirming the conclusion.

c) incorrect 	 It's denying the premise.

d) correct 	 Modus tollens.

##### 17

Wrong ES, $\exist x H(x)$ means there is at least one person who is happy, but it maybe happen that  $H(Lola)$ isn't True (means Lola isn't the happy one).



##### 27

We have:

$1.\forall x (P(x) \rightarrow (Q(x) \and S(x)) )$

$2.\forall x (P(x) \and R(x))$

Then:



| $1$  | $\forall x (P(x) \rightarrow (Q(x) \and S(x)) )$ |     $premise1$     |
| :--: | :----------------------------------------------: | :----------------: |
| $2$  |        $P(c)\rightarrow (Q(c)\land S(c))$        |        US,1        |
| $3$  |           $\forall x(P(x)\land R(x))$            |     $premise2$     |
| $4$  |                 $P(c)\land R(c)$                 |        US,3        |
| $5$  |                     $P( c )$                     | $simplification,4$ |
| $6$  |                 $Q(c)\land S(c)$                 |  $Modus \ Ponens$  |
| $7$  |                      $S(c)$                      | $simplification,6$ |
| $8$  |                 $P(c)\land S(c)$                 | $conjunction,5,7$  |
| $9$  |           $\forall x(P(x)\land S(x))$            |        UG,8        |

